src/program_proof/pav/marshalutil.v
@@ -1,0 +1,44 @@
+From Perennial.program_proof Require Import grove_prelude.
+From Perennial Require Import base.
+From Goose.github_com.mit_pdos.pav Require Import marshalutil.
+
+From Perennial.program_proof Require Import marshal_stateless_proof.
+
+Section wps.
+Context `{!heapGS Σ}.
+
+Definition read_bool (b0 : list w8) : (bool * list w8 * bool) :=
+  match b0 with
+  | [] => (false, [], true)
+  | a :: l => (bool_decide (uint.Z a ≠ 0), l, false)
+  end.
+
+Lemma wp_ReadBool b0_sl dq (b0 : list w8) :
+  let '(v, b, err) := read_bool b0 in
+  {{{ own_slice_small b0_sl byteT dq b0 }}}
+    ReadBool (slice_val b0_sl)
+  {{{
+        sl, RET (#v, slice_val sl, #err);
+        own_slice_small sl byteT dq b
+  }}}.
+Proof.
+  destruct b0; intros ?.
+  - iIntros "Hpre HΦ".
+    wp_rec. wp_apply wp_ref_to; [val_ty|].
+    iIntros (?) "Hb_ptr". wp_pures.
+    iDestruct (own_slice_small_sz with "[$]") as %Hsz.
+    wp_load. wp_apply wp_slice_len. wp_pures.
+    simpl in *. rewrite -> bool_decide_true by word. wp_pures.
+    replace (slice.nil) with (slice_val Slice.nil) by done.
+    iApply "HΦ". iApply own_slice_small_nil. done.
+  - iIntros "Hpre HΦ".
+    wp_rec. wp_apply wp_ref_to; [val_ty|].
+    iIntros (?) "Hb_ptr". wp_pures.
+    iDestruct (own_slice_small_sz with "[$]") as %Hsz.
+    wp_load. wp_apply wp_slice_len. wp_pures.
+    simpl in *. rewrite -> (bool_decide_false (_ < _)) by word. wp_pures.
+    wp_load. wp_apply (wp_ReadBool with "[$]"). iIntros "* [% Hsl]". subst.
+    wp_pures. by iApply "HΦ".
+Qed.
+
+End wps.
